Key_Value_Stores - added some general lemmas about sets, lists, etc - added some lemmas about vl_readers and vl_writers - added [simp] attribute to some ‘obvious’ simplifications - as a result, removed a bunch of trivial lemmas
Serializable_2PC_2PL:
- turned eligible_reads into a definition, now returns a set, not predicate

Serializable_2PC_2PL_Proof:
- repaired sorried proof (some still ugly)
- made many proofs related to SqnInv  more structured, less brute force
- KVSGSNonEmp now derived from KVSNonEmp (implication, not invariant)
- proved additional lemmas about vl_readers and vl_writers (2PC-2PL-dependent)

txn-data-consistency/Serializable_2PC_2PL_Proof.thy
@@ -297,7 +297,7 @@ lemma update_kv_key_reads_all_txn_length [simp]:
 lemma update_kv_key_writes_all_txn_length:
   "length (update_kv_key_writes_all_txn tStm tSkm tFk vl) = Suc (length vl) \<or>
   length (update_kv_key_writes_all_txn tStm tSkm tFk vl) = length vl"
-  by (auto simp add: update_kv_key_writes_all_txn_def update_kv_key_writes_length)
+  by (auto simp add: update_kv_key_writes_all_txn_def)
 
 lemma update_kv_key_writes_all_txn_length_increasing [simp]:
   "length vl \<le> length (update_kv_key_writes_all_txn tStm tSkm tFk vl)"
@@ -308,7 +308,7 @@ lemma update_kv_key_writes_all_txn_on_diff_len:
   shows "length (update_kv_key_writes_all_txn tStm tSkm tFk vl1) \<le>
          length (update_kv_key_writes_all_txn tStm tSkm tFk vl2)"
   using assms
-  by (auto simp add: update_kv_key_writes_all_txn_def update_kv_key_writes_on_diff_len)
+  by (auto simp add: update_kv_key_writes_all_txn_def)
 
 lemma update_kv_all_txn_length:
   "length (update_kv_all_txn tStm tSkm tFk vl) = length vl \<or>
@@ -340,9 +340,8 @@ lemma update_kv_all_txn_non_empty [simp]:
   by (metis update_kv_all_txn_length_increasing le_zero_eq length_0_conv)
 
 lemma read_only_update [simp]:
-  assumes "\<And>t. svr_state (svrs s k) t \<noteq> write_lock"
-  shows "update_kv_all_txn tStm (svr_state (svrs s k)) tFk vl =
-         update_kv_key_reads_all_txn tStm (svr_state (svrs s k)) tFk vl"
+  assumes "\<And>t. tSkm t \<noteq> write_lock"
+  shows "update_kv_all_txn tStm tSkm tFk vl = update_kv_key_reads_all_txn tStm tSkm tFk vl"
   using assms
   by (auto simp add: update_kv_all_txn_def update_kv_key_writes_all_txn_def)
 
@@ -374,18 +373,20 @@ lemma svr_vl_eq_all_k:
 
 lemma eq_for_all_k: 
   assumes "f (svrs s' k) t = f (svrs s k) t"
-    and "\<forall>k'. k' \<noteq> k \<longrightarrow> svrs s' k' = svrs s k'"
-    and "\<forall>t'. t' \<noteq> t \<longrightarrow> f (svrs s' k) t' = f (svrs s k) t'"
-  shows "\<forall>k. f (svrs s' k) = f (svrs s k)"
-  apply (auto simp add: fun_eq_iff) using assms
-  subgoal for k' t' by (cases "k' = k"; cases "t' = t"; simp).
+    and "\<And>k'. k' \<noteq> k \<Longrightarrow> svrs s' k' = svrs s k'"
+    and "\<And>t'. t' \<noteq> t \<Longrightarrow> f (svrs s' k) t' = f (svrs s k) t'"
+  shows "f (svrs s' k) = f (svrs s k)"
+  using assms
+  apply (auto simp add: fun_eq_iff) 
+  subgoal for t' by (cases "t' = t", simp_all)
+  done
 
 lemma eq_for_all_cl:
   assumes "f (cls s' cl) = f (cls s cl)"
     and "\<forall>cl'. cl' \<noteq> cl \<longrightarrow> cls s' cl' = cls s cl'"
-  shows "\<forall>cl. f (cls s' cl) = f (cls s cl)"
-  apply (auto simp add: fun_eq_iff) using assms
-  subgoal for cl' by (cases "cl' = cl"; simp).
+  shows "f (cls s' cl') = f (cls s cl')"
+  using assms 
+  by (cases "cl' = cl"; simp)
 
 lemma other_sn_idle:  
   assumes "TIDFutureKm s cl" and "TIDPastKm s cl"
@@ -581,32 +582,21 @@ next
   then show ?case
   proof (induction e)
     case (Commit x1 x2)
-    then show ?case using reach_trans      
+    then show ?case using reach_trans 
       by (auto simp add: KVSNonEmp_def tps_trans_defs svr_unchanged_defs)
-         (metis longer_list_not_empty update_kv_key_length_increasing)+
+         (metis length_greater_0_conv list.size(3) nat.distinct(1) length_update_kv_key)+
   qed (auto simp add: KVSNonEmp_def tps_trans_defs unchanged_defs dest!: svr_vl_eq_all_k)
 qed
 
-definition KVSGSNonEmp where
+definition KVSGSNonEmp where    
   "KVSGSNonEmp s \<longleftrightarrow> (\<forall>k. kvs_of_gs s k \<noteq> [])"
 
 lemmas KVSGSNonEmpI = KVSGSNonEmp_def[THEN iffD2, rule_format]
 lemmas KVSGSNonEmpE[elim] = KVSGSNonEmp_def[THEN iffD1, elim_format, rule_format]
 
-lemma reach_kvs_gs_non_emp [simp, dest]:
-  assumes "reach tps s"
-    and "KVSNonEmp s"
-  shows "KVSGSNonEmp s"
-  using assms
-proof(induction s rule: reach.induct)
-  case (reach_init s)
-  then show ?case
-    by (auto simp add: KVSGSNonEmp_def kvs_of_gs_def tps_defs)
-next
-  case (reach_trans s e s')
-  then show ?case
-    by (induction e) (auto simp add: KVSGSNonEmp_def tps_trans_defs kvs_of_gs_def unchanged_defs)
-qed
+lemma kvs_non_mp_implies_kvs_gs_non_emp [simp, dest]: "KVSNonEmp s \<Longrightarrow> KVSGSNonEmp s"
+  by (auto simp add: KVSGSNonEmp_def kvs_of_gs_def)
+
 
 subsubsection \<open>Lemmas for kvs_of_gs changing by different events\<close>
 
@@ -620,9 +610,10 @@ lemma eligible_reads_svr_inv:
           cl_state (cls s (get_cl t)) \<noteq> cl_committed"
     and "cl_svr_k'_t'_unchanged k s s' t"
   shows "
-  eligible_reads (\<lambda>t. cl_state (cls s' (get_cl t))) (svr_state (svrs s' k)) (svr_fp (svrs s' k)) t' =
-  eligible_reads (\<lambda>t. cl_state (cls s (get_cl t))) (svr_state (svrs s k)) (svr_fp (svrs s k)) t'"
-  using assms apply (cases "t' = t"; simp add: svr_unchanged_defs) by metis
+  eligible_reads (\<lambda>t. cl_state (cls s' (get_cl t))) (svr_state (svrs s' k)) (svr_fp (svrs s' k)) =
+  eligible_reads (\<lambda>t. cl_state (cls s (get_cl t))) (svr_state (svrs s k)) (svr_fp (svrs s k))"
+  using assms apply (auto simp add: eligible_reads_def svr_unchanged_defs) 
+  by metis+
 
 lemma none_eligible: "vl[Max (full_view vl) := last_version vl (full_view vl)
   \<lparr>v_readerset := v_readerset (last_version vl (full_view vl)) \<union> {}\<rparr>] = vl"
@@ -633,23 +624,24 @@ lemma eligible_reads_read_lock_inv:
     and "svr_state (svrs s k) t = read_lock"
     and "cl_state (cls s (get_cl t)) = cl_committed"
     and "cl_svr_k'_t'_unchanged k s s' t"
-  shows "{t. eligible_reads (\<lambda>t. cl_state (cls s (get_cl t))) (svr_state (svrs s k))
-            (svr_fp (svrs s k)) t} =
-          insert t {t. eligible_reads (\<lambda>t. cl_state (cls s (get_cl t))) (svr_state (svrs s' k))
-            (svr_fp (svrs s k)) t}"
-  using assms by (auto simp add: svr_unchanged_defs)
+  shows "eligible_reads (\<lambda>t. cl_state (cls s (get_cl t))) (svr_state (svrs s k))
+            (svr_fp (svrs s k)) =
+          insert t (eligible_reads (\<lambda>t. cl_state (cls s (get_cl t))) (svr_state (svrs s' k))
+            (svr_fp (svrs s k)))"
+  using assms by (auto simp add: eligible_reads_def svr_unchanged_defs)
 
 lemma eligible_reads_write_lock_s_the_t:
   assumes "RLockInv s k" and "WLockInv s k"
     and "svr_state (svrs s k) t = write_lock"
     and "cl_state (cls s (get_cl t)) = cl_committed"
     and "cl_svr_k'_t'_unchanged k s s' t"
-  shows "{t. eligible_reads (\<lambda>t. cl_state (cls s (get_cl t))) (svr_state (svrs s k))
-            (svr_fp (svrs s k)) t} =
+  shows "eligible_reads (\<lambda>t. cl_state (cls s (get_cl t))) (svr_state (svrs s k))
+            (svr_fp (svrs s k)) =
          (case (svr_fp (svrs s k) t R) of None \<Rightarrow> {} | Some y \<Rightarrow> {t})"
   using assms
-  apply (auto intro: Collect_empty_eq split: option.split)
-  subgoal for t' by (cases "t' = t"; auto simp add: RLockInv_def WLockInv_def svr_unchanged_defs).
+  apply (auto simp add: eligible_reads_def intro: Collect_empty_eq split: option.split)
+  subgoal for t' by (cases "t' = t"; auto simp add: RLockInv_def WLockInv_def svr_unchanged_defs)
+  done
 
 lemma update_kv_key_reads_commit_w_s_inv:
   assumes "RLockInv s k" and "WLockInv s k"
@@ -669,12 +661,13 @@ lemma eligible_reads_write_lock_s'_empty:
     and "svr_state (svrs s k) t = write_lock"
     and "svr_state (svrs s' k) t = committed"
     and "cl_svr_k'_t'_unchanged k s s' t"
-  shows "{t. eligible_reads (\<lambda>t. cl_state (cls s (get_cl t))) (svr_state (svrs s' k))
-            (svr_fp (svrs s k)) t} = {}"
+  shows "eligible_reads (\<lambda>t. cl_state (cls s (get_cl t))) (svr_state (svrs s' k))
+            (svr_fp (svrs s k)) = {}"
   using assms
-  apply (auto intro: Collect_empty_eq)
+  apply (auto simp add: eligible_reads_def intro: Collect_empty_eq)
   subgoal for t' by (cases "t' = t"; auto simp add: RLockInv_def WLockInv_def svr_unchanged_defs)
-  subgoal for t' by (cases "t' = t"; auto simp add: RLockInv_def WLockInv_def svr_unchanged_defs).
+  subgoal for t' by (cases "t' = t"; auto simp add: RLockInv_def WLockInv_def svr_unchanged_defs)
+  done
 
 lemma update_kv_key_reads_commit_w_s'_inv:
   assumes "RLockInv s k" and "WLockInv s k"
@@ -692,9 +685,9 @@ lemma eligible_reads_no_lock_inv:
     and "svr_state (svrs s' k) t = committed"
     and "cl_svr_k'_t'_unchanged k s s' t"
   shows "
-  eligible_reads (\<lambda>t. cl_state (cls s (get_cl t))) (svr_state (svrs s' k)) (svr_fp (svrs s k)) t' =
-  eligible_reads (\<lambda>t. cl_state (cls s (get_cl t))) (svr_state (svrs s k)) (svr_fp (svrs s k)) t'"
-  using assms apply (auto simp add: svr_unchanged_defs)
+  eligible_reads (\<lambda>t. cl_state (cls s (get_cl t))) (svr_state (svrs s' k)) (svr_fp (svrs s k)) =
+  eligible_reads (\<lambda>t. cl_state (cls s (get_cl t))) (svr_state (svrs s k)) (svr_fp (svrs s k))"
+  using assms apply (auto simp add: eligible_reads_def svr_unchanged_defs)
   apply (metis state_svr.distinct(33))
   apply (metis state_svr.distinct(41))
   apply (metis state_svr.distinct(29))
@@ -785,16 +778,16 @@ lemma eligible_reads_cl_inv:
     and "cl_state (cls s' cl) \<noteq> cl_committed"
     and "svr_cl_cl'_unchanged cl s s'"
   shows "
-  eligible_reads (\<lambda>t. cl_state (cls s' (get_cl t))) (svr_state (svrs s k)) (svr_fp (svrs s k)) t =
-  eligible_reads (\<lambda>t. cl_state (cls s (get_cl t))) (svr_state (svrs s k)) (svr_fp (svrs s k)) t"
-  using assms apply (auto simp add: update_kv_key_writes_all_txn_def cl_unchanged_defs)
-  subgoal
+  eligible_reads (\<lambda>t. cl_state (cls s' (get_cl t))) (svr_state (svrs s k)) (svr_fp (svrs s k)) =
+  eligible_reads (\<lambda>t. cl_state (cls s (get_cl t))) (svr_state (svrs s k)) (svr_fp (svrs s k))"
+  using assms apply (auto simp add: eligible_reads_def cl_unchanged_defs)
+  subgoal for t v
     apply (cases "get_cl t = cl"; cases "get_sn t = cl_sn (cls s cl)";
             simp add: cl_unchanged_defs)
     apply (metis txid0.collapse state_svr.distinct(33))
     by (metis empty_iff insert_iff other_sn_idle state_svr.distinct(3)
         state_svr.distinct(33) state_svr.distinct(35))
-  subgoal
+  subgoal for t v
     apply (cases "get_cl t = cl"; cases "get_sn t = cl_sn (cls s cl)";
             simp add: cl_unchanged_defs)
     apply (metis txid0.collapse state_svr.distinct(41))
@@ -809,12 +802,18 @@ lemma eligible_reads_cl_commit_no_lock_inv:
     and "other_insts_unchanged cl (cls s) (cls s')"
     and "svr_state (svrs s k) (get_txn cl s) = no_lock"
   shows "
-  eligible_reads (\<lambda>t. cl_state (cls s' (get_cl t))) (svr_state (svrs s k)) (svr_fp (svrs s k)) t =
-  eligible_reads (\<lambda>t. cl_state (cls s (get_cl t))) (svr_state (svrs s k)) (svr_fp (svrs s k)) t"
-  using assms apply (cases "get_cl t = cl"; simp add: other_insts_unchanged_def)
-  by (metis empty_iff txid0.collapse insert_iff other_sn_idle
-      state_svr.distinct(29) state_svr.distinct(3) state_svr.distinct(33) state_svr.distinct(35)
-      state_svr.distinct(37) state_svr.distinct(41) state_svr.distinct(43) state_svr.distinct(5))
+  eligible_reads (\<lambda>t. cl_state (cls s' (get_cl t))) (svr_state (svrs s k)) (svr_fp (svrs s k)) =
+  eligible_reads (\<lambda>t. cl_state (cls s (get_cl t))) (svr_state (svrs s k)) (svr_fp (svrs s k))"
+  using assms 
+  apply (auto simp add: eligible_reads_def other_insts_unchanged_def)
+  subgoal for t v
+    by (metis insertE other_sn_idle singleton_iff state_svr.distinct(3) state_svr.distinct(35) 
+              state_svr.simps(30) state_svr.simps(34) txid0.collapse) 
+  subgoal for t v
+    by (metis insertE other_sn_idle singleton_iff state_svr.distinct(5) state_svr.simps(38) 
+              state_svr.simps(42) state_svr.simps(44) txid0.collapse)
+  done
+
 
 \<comment> \<open>write updates\<close>
 lemma update_kv_key_writes_cl_inv:
@@ -825,7 +824,7 @@ lemma update_kv_key_writes_cl_inv:
     and "svr_cl_cl'_unchanged cl s s'"
   shows "update_kv_key_writes_all_txn (\<lambda>t. cl_state (cls s' (get_cl t)))
                 (svr_state (svrs s k)) (svr_fp (svrs s k)) vl =
-               update_kv_key_writes_all_txn (\<lambda>t. cl_state (cls s (get_cl t)))
+         update_kv_key_writes_all_txn (\<lambda>t. cl_state (cls s (get_cl t)))
                 (svr_state (svrs s k)) (svr_fp (svrs s k)) vl"
   using assms apply (auto simp add: update_kv_key_writes_all_txn_def cl_unchanged_defs)
   subgoal for t
@@ -859,13 +858,17 @@ lemma update_kv_all_cl_commit_no_lock_inv:
           (svr_fp (svrs s k)) (svr_vl (svrs s k))"
   using assms eligible_reads_cl_commit_no_lock_inv[of s cl s' k]
   apply (auto simp add: NoLockFpInv_def update_kv_all_defs other_insts_unchanged_def)
-  apply (metis (mono_tags, lifting) txid0.collapse insert_compr mem_Collect_eq other_sn_idle singleton_conv2
+  by (metis (mono_tags, lifting) txid0.collapse insert_compr mem_Collect_eq other_sn_idle singleton_conv2
                state_svr.distinct(37) state_svr.distinct(41) state_svr.distinct(43) state_svr.distinct(5))
-  by metis
 
 (*All events*)
-abbreviation not_cl_commit where
-  "not_cl_commit e \<equiv> \<forall>cl sn u'' F. e \<noteq> Cl_Commit cl sn u'' F"
+fun not_cl_commit :: "'a ev \<Rightarrow> bool" where
+  "not_cl_commit (Cl_Commit cl sn u'' F) = False" |
+  "not_cl_commit _ = True"
+
+lemma not_not_cl_commit [simp]: "\<not>not_cl_commit e \<longleftrightarrow> (\<exists>cl sn u'' F. e = Cl_Commit cl sn u'' F)" 
+  by (auto elim: not_cl_commit.elims)
+
 
 abbreviation invariant_list_kvs where
   "invariant_list_kvs s \<equiv> \<forall>cl k. TIDFutureKm s cl \<and> TIDPastKm s cl \<and> RLockInv s k \<and> WLockInv s k \<and>
@@ -877,83 +880,89 @@ lemma kvs_of_gs_inv:
     and "not_cl_commit e"
   shows "kvs_of_gs s' = kvs_of_gs s"
   using assms
-  proof (induction e)
-    case (Prepare x1 x2)
-    then show ?case using kvs_of_gs_svr_inv[of s x1 s' x2]
-      by (auto simp add: tps_trans_defs svr_unchanged_defs dest!: svr_vl_eq_all_k)
-  next
-    case (RLock x1 x2 x3)
-    then show ?case using kvs_of_gs_svr_inv[of s x1 s' x3]
-      by (auto simp add: tps_trans_defs svr_unchanged_defs dest!: svr_vl_eq_all_k)
-  next
-    case (WLock x1 x2 x3 x4)
-    then show ?case using kvs_of_gs_svr_inv[of s x1 s' x4]
-      by (auto simp add: tps_trans_defs svr_unchanged_defs dest!: svr_vl_eq_all_k)
-  next
-    case (NoLock x1 x2)
-    then show ?case using kvs_of_gs_svr_inv[of s x1 s' x2]
-      by (auto simp add: tps_trans_defs svr_unchanged_defs dest!: svr_vl_eq_all_k)
-  next
-    case (NOK x1 x2)
-    then show ?case using kvs_of_gs_svr_inv[of s x1 s' x2]
-      by (auto simp add: tps_trans_defs svr_unchanged_defs dest!: svr_vl_eq_all_k)
-  next
-    case (Commit x1 x2)
-    hence u: "kvs_of_gs s' x1 = kvs_of_gs s x1"
-      apply (auto simp add: kvs_of_gs_def commit_def)
-      subgoal
-        using eligible_reads_read_lock_inv[of s x1 x2 s']
-              update_kv_key_writes_commit_r_inv[of s x1 x2 s']
-        apply (auto simp add: update_kv_all_txn_def update_kv_key_reads_all_txn_def Let_def
-                              svr_unchanged_defs)
-        (* SH does not work *)
-        sorry 
-
-        thm eq_for_all_k  
-        thm update_kv_key_ro_set_v_readerset
-
-(* does not terminate?
-        by (auto simp add: update_kv_all_txn_def update_kv_key_reads_all_txn_def Let_def
-            RLockFpInv_def KVSNonEmp_def svr_unchanged_defs update_kv_key_ro_set_v_readerset
-            dest!: eq_for_all_k)
-*)
-      subgoal
-        using update_kv_key_reads_commit_w_s_inv[of s x1 x2 s']
-              update_kv_key_reads_commit_w_s'_inv[of s x1 x2 s']
-              update_kv_key_writes_commit_w_s_inv[of s x1 x2 s']
-              update_kv_key_writes_commit_w_s'_inv[of s x1 x2 s']
-        by (auto simp add: update_kv_all_txn_def update_kv_key_def Let_def
-            svr_unchanged_defs dest!: eq_for_all_k split: option.split)
-      subgoal
-        using eligible_reads_no_lock_inv[of s x1 x2 s']
-        using update_kv_key_writes_commit_n_inv[of s x1 x2 s']
-        by (auto simp add: update_kv_all_txn_def update_kv_key_reads_all_txn_def
-            NoLockFpInv_def svr_unchanged_defs dest!: eq_for_all_k) 
+proof (induction e)
+  case (Prepare x1 x2)
+  then show ?case using kvs_of_gs_svr_inv[of s x1 s' x2]
+    by (auto simp add: tps_trans_defs svr_unchanged_defs dest!: svr_vl_eq_all_k)
+next
+  case (RLock x1 x2 x3)
+  then show ?case using kvs_of_gs_svr_inv[of s x1 s' x3]
+    by (auto simp add: tps_trans_defs svr_unchanged_defs dest!: svr_vl_eq_all_k)
+next
+  case (WLock x1 x2 x3 x4)
+  then show ?case using kvs_of_gs_svr_inv[of s x1 s' x4]
+    by (auto simp add: tps_trans_defs svr_unchanged_defs dest!: svr_vl_eq_all_k)
+next
+  case (NoLock x1 x2)
+  then show ?case using kvs_of_gs_svr_inv[of s x1 s' x2]
+    by (auto simp add: tps_trans_defs svr_unchanged_defs dest!: svr_vl_eq_all_k)
+next
+  case (NOK x1 x2)
+  then show ?case using kvs_of_gs_svr_inv[of s x1 s' x2]
+    by (auto simp add: tps_trans_defs svr_unchanged_defs dest!: svr_vl_eq_all_k)
+next
+  case (Commit k t)
+  hence u: "kvs_of_gs s' k = kvs_of_gs s k"
+    apply (auto simp add: kvs_of_gs_def commit_def)
+    subgoal 
+      using eligible_reads_read_lock_inv[of s k t s']
+            update_kv_key_writes_commit_r_inv[of s k t s']
+      apply (auto simp add: update_kv_all_txn_def update_kv_key_reads_all_txn_def Let_def
+               RLockFpInv_def KVSNonEmp_def svr_unchanged_defs update_kv_key_ro_set_v_readerset
+               dest!: eq_for_all_k[where f=svr_fp])   (* loops if not instantiated *)
+      (* 
+        previous apply is unable to use the RLockFpInv: 
+        there is a problem with the way invariants are used here. 
+      *)
+      apply (drule spec[where x=undefined], clarsimp)  (* what else? there is no free cl here! *)
+      apply (rotate_tac -1)
+      apply (drule spec[where x=k], clarsimp)
+      apply (rotate_tac -3)
+      apply (drule spec[where x=t], clarsimp)
       done
-    hence "\<forall>k. k \<noteq> x1 \<longrightarrow> kvs_of_gs s' k = kvs_of_gs s k" using Commit
-      by (auto simp add: commit_def svr_unchanged_defs kvs_of_gs_def)
-    then show ?case using u by auto
-  next
-    case (Abort x1 x2)
-    then show ?case using kvs_of_gs_svr_inv[of s x1 s' x2]
-      by (auto simp add: tps_trans_defs svr_unchanged_defs dest!: svr_vl_eq_all_k)
-  next
-    case (User_Commit x)
-    then show ?case using kvs_of_gs_cl_inv[of s x s']
-     by (auto simp add: tps_trans_defs cl_unchanged_defs)
-  next
-    case (Cl_Abort x)
-    then show ?case using kvs_of_gs_cl_inv[of s x s']
-     by (auto simp add: tps_trans_defs cl_unchanged_defs)
-  next
-    case (Cl_ReadyC x)
-    then show ?case using kvs_of_gs_cl_inv[of s x s']
-     by (auto simp add: tps_trans_defs cl_unchanged_defs)
-  next
-    case (Cl_ReadyA x)
-    then show ?case using kvs_of_gs_cl_inv[of s x s']
-     by (auto simp add: tps_trans_defs cl_unchanged_defs)
- qed auto
+
+(* loops:
+      by (auto simp add: update_kv_all_txn_def update_kv_key_reads_all_txn_def Let_def
+               RLockFpInv_def KVSNonEmp_def svr_unchanged_defs update_kv_key_ro_set_v_readerset
+               dest!: eq_for_all_k)
+*)
+    subgoal
+        using update_kv_key_reads_commit_w_s_inv[of s k t s']
+              update_kv_key_reads_commit_w_s'_inv[of s k t s']
+              update_kv_key_writes_commit_w_s_inv[of s k t s']
+              update_kv_key_writes_commit_w_s'_inv[of s k t s']
+        by (auto simp add: update_kv_all_txn_def update_kv_key_def Let_def
+            svr_unchanged_defs dest: eq_for_all_k split: option.split)
+    subgoal 
+        using eligible_reads_no_lock_inv[of s k t s']
+        using update_kv_key_writes_commit_n_inv[of s k t s']
+        by (auto simp add: update_kv_all_txn_def update_kv_key_reads_all_txn_def
+            NoLockFpInv_def svr_unchanged_defs dest: eq_for_all_k) 
+    done
+  hence "\<forall>k'. k' \<noteq> k \<longrightarrow> kvs_of_gs s' k' = kvs_of_gs s k'" using Commit
+    by (auto simp add: commit_def svr_unchanged_defs kvs_of_gs_def)
+  then show ?case using u by auto
+next
+  case (Abort x1 x2)
+  then show ?case using kvs_of_gs_svr_inv[of s x1 s' x2]
+    by (auto simp add: tps_trans_defs svr_unchanged_defs dest!: svr_vl_eq_all_k)
+next
+  case (User_Commit x)
+  then show ?case using kvs_of_gs_cl_inv[of s x s']
+   by (auto simp add: tps_trans_defs cl_unchanged_defs)
+next
+  case (Cl_Abort x)
+  then show ?case using kvs_of_gs_cl_inv[of s x s']
+   by (auto simp add: tps_trans_defs cl_unchanged_defs)
+next
+  case (Cl_ReadyC x)
+  then show ?case using kvs_of_gs_cl_inv[of s x s']
+   by (auto simp add: tps_trans_defs cl_unchanged_defs)
+next
+  case (Cl_ReadyA x)
+  then show ?case using kvs_of_gs_cl_inv[of s x s']
+    by (auto simp add: tps_trans_defs cl_unchanged_defs)
+qed auto
 
 \<comment> \<open>More specific lemmas about TM commit\<close>
 lemma kvs_of_gs_commit_length_increasing:
@@ -962,25 +971,30 @@ lemma kvs_of_gs_commit_length_increasing:
     and "svr_cl_cl'_unchanged cl s s'"
   shows "length (kvs_of_gs s k) \<le> length (kvs_of_gs s' k)"
   using assms
-  apply (auto simp add: kvs_of_gs_def cl_unchanged_defs update_kv_all_txn_def
-      update_kv_key_writes_all_txn_def update_kv_key_writes_on_diff_len)
-  by (metis (no_types, lifting) update_kv_key_reads_all_txn_length update_kv_key_writes_length_increasing)
+  by (force simp add: kvs_of_gs_def cl_unchanged_defs update_kv_all_txn_def
+                      update_kv_key_writes_all_txn_def)
 
 lemma kvs_of_gs_length_increasing:
   assumes "gs_trans s e s'"
     and "invariant_list_kvs s"
-  shows "\<And>k. length (kvs_of_gs s k) \<le> length (kvs_of_gs s' k)"
-  using assms
-  apply (cases "not_cl_commit e"; simp add: kvs_of_gs_inv)
-  apply auto apply (simp add: cl_commit_def) by (auto dest!: kvs_of_gs_commit_length_increasing)
+  shows "length (kvs_of_gs s k) \<le> length (kvs_of_gs s' k)"
+proof (cases "not_cl_commit e")
+  case True
+  then show ?thesis using assms by (simp add: kvs_of_gs_inv)
+next
+  case False
+  then show ?thesis using assms(1) 
+    by (auto simp add: cl_commit_def kvs_of_gs_commit_length_increasing)
+qed
+
 
 lemma cl_commit_expands_eligible_reads:
   assumes "cl_state (cls s' cl) = cl_committed"
     and "other_insts_unchanged cl (cls s) (cls s')"
   shows
-  "{t. eligible_reads (\<lambda>t. cl_state (cls s (get_cl t))) (svr_state (svrs s k)) (svr_fp (svrs s k)) t} \<subseteq>
-   {t. eligible_reads (\<lambda>t. cl_state (cls s' (get_cl t))) (svr_state (svrs s k)) (svr_fp (svrs s k)) t}"
-  using assms by (auto simp add: other_insts_unchanged_def)
+  "eligible_reads (\<lambda>t. cl_state (cls s (get_cl t))) (svr_state (svrs s k)) (svr_fp (svrs s k)) \<subseteq>
+   eligible_reads (\<lambda>t. cl_state (cls s' (get_cl t))) (svr_state (svrs s k)) (svr_fp (svrs s k))"
+  using assms by (auto simp add: eligible_reads_def other_insts_unchanged_def)
 
 lemma cl_commit_expands_eligible_reads':
   assumes "NoLockFpInv s k" and "TIDPastKm s cl" and "TIDFutureKm s cl"
@@ -988,22 +1002,21 @@ lemma cl_commit_expands_eligible_reads':
     and "cl_state (cls s' cl) = cl_committed"
     and "is_locked (svr_state (svrs s k) (get_txn cl s))"
     and "other_insts_unchanged cl (cls s) (cls s')"
-  shows "{x. eligible_reads (\<lambda>t. cl_state (cls s' (get_cl t))) (svr_state (svrs s k))
-    (svr_fp (svrs s k)) x} = (case svr_fp (svrs s k) (get_txn cl s) R of
-   None \<Rightarrow> {x. eligible_reads (\<lambda>t. cl_state (cls s (get_cl t))) (svr_state (svrs s k))
-     (svr_fp (svrs s k)) x}|
-   Some _ \<Rightarrow> insert (get_txn cl s) {x. eligible_reads (\<lambda>t. cl_state (cls s (get_cl t)))
-     (svr_state (svrs s k)) (svr_fp (svrs s k)) x})"
+  shows 
+    "eligible_reads (\<lambda>t. cl_state (cls s' (get_cl t))) (svr_state (svrs s k)) (svr_fp (svrs s k)) 
+     = (case svr_fp (svrs s k) (get_txn cl s) R of
+   None \<Rightarrow> eligible_reads (\<lambda>t. cl_state (cls s (get_cl t))) (svr_state (svrs s k))
+     (svr_fp (svrs s k)) |
+   Some _ \<Rightarrow> insert (get_txn cl s) (eligible_reads (\<lambda>t. cl_state (cls s (get_cl t)))
+     (svr_state (svrs s k)) (svr_fp (svrs s k))))"
   using assms
-  apply (auto simp add: other_insts_unchanged_def NoLockFpInv_def split: option.split del: disjE)
-  subgoal for t apply (cases "get_cl t = cl"; cases "get_sn t = cl_sn (cls s cl)"; simp)
-    apply (metis txid0.collapse option.distinct(1))
-    by (metis emptyE insert_iff other_sn_idle state_svr.distinct(3) state_svr.distinct(33)
-        state_svr.distinct(35) state_svr.distinct(41) state_svr.distinct(43) state_svr.distinct(5))
-  subgoal for v t apply (cases "get_cl t = cl"; cases "get_sn t = cl_sn (cls s cl)"; simp)
-    apply (metis txid0.collapse)
-    by (metis empty_iff insertE other_sn_idle state_svr.distinct(3) state_svr.distinct(33)
-        state_svr.distinct(35) state_svr.distinct(41) state_svr.distinct(43) state_svr.distinct(5))
+  apply (auto simp add: eligible_reads_def other_insts_unchanged_def NoLockFpInv_def 
+              split: option.split del: disjE)
+  subgoal
+    by (metis insertE option.discI other_sn_idle singletonD state_svr.distinct(3,5,33,35,41,43)  
+              txid0.collapse)
+  subgoal
+    by (metis insertE other_sn_idle singletonD state_svr.distinct(3,5,34,36,42,44) txid0.collapse) 
   by auto
   
 lemma cl_commit_updates_kv_reads:
@@ -1063,6 +1076,7 @@ lemma cl_commit_writer_update_kv_all:
 
 \<comment> \<open>Fingerprint content invariant and Lemmas for proving the fp_property\<close>
 
+(* no longer used:
 lemma svr_vl_read_lock_commit_eq_length:
   assumes "RLockFpInv s k"
     and "svr_state (svrs s k) t = read_lock"
@@ -1070,8 +1084,8 @@ lemma svr_vl_read_lock_commit_eq_length:
           update_kv_key t (svr_fp (svrs s k) t) (full_view (svr_vl (svrs s k))) (svr_vl (svrs s k))"
   shows "length (svr_vl (svrs s' k)) = length (svr_vl (svrs s k))"
   using assms
-  by (auto simp add: RLockFpInv_def update_kv_key_length)
-
+  by (auto)
+*)
 lemma svr_vl_read_commit_eq_lv:
   assumes "RLockFpInv s k"
     and "svr_state (svrs s k) t = read_lock"
@@ -1080,8 +1094,9 @@ lemma svr_vl_read_commit_eq_lv:
           update_kv_key t (svr_fp (svrs s k) t) (full_view (svr_vl (svrs s k))) (svr_vl (svrs s k))"
   shows "v_value (last_version (svr_vl (svrs s' k)) (full_view (svr_vl (svrs s' k)))) =
          v_value (last_version (svr_vl (svrs s k)) (full_view (svr_vl (svrs s k))))"
-  using assms svr_vl_read_lock_commit_eq_length[of s k t s']
-  by (metis full_view_def max_in_full_view update_kv_key_v_value_inv)
+  using assms
+  by (metis RLockFpInv_def max_in_full_view full_view_update_kv_key_no_write update_kv_key_v_value_inv)
+
 
 definition RLockFpContentInv where
   "RLockFpContentInv s k \<longleftrightarrow> (\<forall>t. svr_state (svrs s k) t = read_lock \<longrightarrow>
@@ -1240,16 +1255,16 @@ lemma updated_vl_view_grows:
     update_kv_key t (svr_fp (svrs s k) t) (full_view (svr_vl (svrs s k))) (svr_vl (svrs s k))"
     and "other_insts_unchanged k (svrs s) (svrs s')"
   shows "(\<lambda>k. full_view (svr_vl (svrs s k))) \<sqsubseteq> (\<lambda>k. full_view (svr_vl (svrs s' k)))"
-  using assms update_kv_key_length_increasing[of "svr_vl (svrs s k)" t "svr_fp (svrs s k) t"
-      "full_view (svr_vl (svrs s k))"]
-  apply (auto simp add: view_order_def other_insts_unchanged_def)
-  by (metis full_view_length_increasing)
+  using assms 
+  by (auto simp add: view_order_def other_insts_unchanged_def)
+     (metis insert_iff full_view_update_kv_key_no_write full_view_update_kv_key_write)
 
 lemma cl_view_inv:
   assumes "gs_trans s e s'"
     and "not_cl_commit e"
   shows "cl_view (cls s' cl) = cl_view (cls s cl)"
-  using assms by (induction e) (auto simp add: tps_trans_defs unchanged_defs dest!:eq_for_all_cl)
+  using assms 
+  by (induction e) (auto simp add: tps_trans_defs unchanged_defs dest: eq_for_all_cl)
 
 lemma updated_is_kvs_of_gs':
   assumes "cl_state (cls s' cl) = cl_committed"
@@ -1285,21 +1300,20 @@ next
     by (metis (no_types, lifting) view_order_refl view_order_trans)
 qed
 
+
+(********************************************************************************************)
+(********************************************************************************************)
+(********************************************************************************************)
+
 \<comment> \<open>Cl_commit updating kv\<close>
 
-lemma or3_not_eq:
-  assumes "\<forall>k. P k = a \<or> P k = b \<or> P k = c"
-    and "P k \<noteq> c"
-  shows "P k = a \<or> P k = b"
-  using assms by auto
-
-lemma kvs_of_gs_cl_commit:
+lemma kvs_of_gs_cl_commit:    (* TODO: check where used and whether generalizable *)
   assumes "TIDFutureKm s cl" and "TIDPastKm s cl"
     and "WLockInv s k" and "WLockFpInv s k"
     and "RLockInv s k" and "RLockFpInv s k"
     and "NoLockFpInv s k" and "KVSNonEmp s"
-    and "cl_state (cls s cl) = cl_prepared"
     and "is_locked (svr_state (svrs s k) (get_txn cl s))"
+    and "cl_state (cls s cl) = cl_prepared"
     and "cl_state (cls s' cl) = cl_committed"
     and "other_insts_unchanged cl (cls s) (cls s')"
   shows "update_kv_all_txn (\<lambda>t. cl_state (cls s' (get_cl t))) (svr_state (svrs s k))
@@ -1318,14 +1332,223 @@ lemma kvs_of_gs_cl_commit:
     by (auto simp add: update_kv_all_txn_def update_kv_key_writes_all_txn_def the_wr_tI)
   by (auto simp add: update_kv_all_cl_commit_no_lock_inv)
 
-\<comment> \<open>Lemmas about reader and writer transaction sets\<close>
-lemma update_kv_key_writes_all_txn_v_readerset_set:
+
+(********************************************************************************************)
+(********************************************************************************************)
+(********************************************************************************************)
+
+
+\<comment> \<open>Lemmas about reader and writer transaction id sets (2PC+2PL)\<close>
+
+text \<open>Readers\<close>
+
+lemma vl_readers_update_kv_key_writes_all_txn [simp]:
   "vl_readers (update_kv_key_writes_all_txn tStm tSkm tFk vl) = vl_readers vl"
-  by (auto simp add: update_kv_key_writes_all_txn_def vl_readers_update_kv_key_writes)
+  by (auto simp add: update_kv_key_writes_all_txn_def)
+
+lemma vl_readers_update_kv_key_reads_all_txn [simp]:
+  assumes "vl \<noteq> []"
+  shows "vl_readers (update_kv_key_reads_all_txn tStm tSkm tFk vl) = 
+         vl_readers vl \<union> eligible_reads tStm tSkm tFk"
+  using assms 
+  apply (auto simp add: update_kv_key_reads_all_txn_def vl_readers_def Let_def full_view_def 
+                        Max_list_index_set set_update del: equalityI)
+  apply (simp add: Un_commute)
+  apply (subst Un_assoc) 
+  apply (intro arg_cong[where f="(\<union>) (eligible_reads tStm tSkm tFk)"])
+  apply auto
+  subgoal by (meson diff_Suc_less length_greater_0_conv nth_mem)
+  subgoal using nth_mem by blast
+  subgoal by (metis in_set_conv_nth)
+  done
+
+lemma vl_readers_update_kv_all_txn [simp]:
+  assumes "vl \<noteq> []"
+  shows "vl_readers (update_kv_all_txn tCls tSvrs tFk vl) = 
+         vl_readers vl \<union> eligible_reads tCls tSvrs tFk"
+  using assms
+  by (auto simp add: update_kv_all_txn_def del: equalityI)
+
+
+text \<open>Readers' sequence numbers\<close>
+(*
+lemma vl_readers_sqns_update_key_reads_all_txn [simp]:
+  assumes "vl \<noteq> []"
+  shows "vl_readers_sqns (update_kv_key_reads_all_txn tCls tSvrs tFk vl) cl = 
+         vl_readers_sqns vl cl \<union> {n. Tn_cl n cl \<in> eligible_reads tCls tSvrs tFk}"
+  using assms
+  by (auto simp add: vl_readers_sqns_def)
+
+lemma vl_readers_sqns_update_kv_key_writes_all_txn [simp]:
+  "vl_readers_sqns (update_kv_key_writes_all_txn tStm tSkm tFk vl) = vl_readers_sqns vl"
+  by (auto simp add: vl_readers_sqns_def)
+*)
+
+lemma vl_readers_sqns_update_kv_all_txn [simp]:
+  assumes "vl \<noteq> []"
+  shows "vl_readers_sqns (update_kv_all_txn tCls tSvrs tFk vl) cl = 
+         vl_readers_sqns vl cl \<union> {n. Tn_cl n cl \<in> eligible_reads tCls tSvrs tFk}"
+  using assms
+  by (auto simp add: vl_readers_sqns_def)
+
+
+text \<open>Writers\<close>
+
+lemma vl_writers_update_kv_key_reads_all_txn [simp]:
+  assumes "vl \<noteq> []"                     
+  shows "vl_writers (update_kv_key_reads_all_txn tCls tSvrs tFk vl) = vl_writers vl"
+  using assms
+  apply (auto simp add: update_kv_key_reads_all_txn_def vl_writers_def Let_def full_view_def 
+                        Max_list_index_set intro!: image_set_equality_iff)
+  subgoal for i by (cases "i = length vl - 1") (auto)
+  done
+
+lemma vl_writers_update_kv_key_writes_all_txn [simp]:
+  assumes "\<And>t. tSvrs t = write_lock \<Longrightarrow> (\<exists>!t. tSvrs t = write_lock)"
+  shows "vl_writers (update_kv_key_writes_all_txn tCls tSvrs tFk vl) = 
+        (if (\<exists>t. tCls t = cl_committed \<and> tSvrs t = write_lock \<and> tFk t W \<noteq> None) 
+         then insert (Tn (the_wr_t tSvrs)) (vl_writers vl) 
+         else vl_writers vl)"
+proof (cases "\<exists>t. tCls t = cl_committed \<and> tSvrs t = write_lock \<and> tFk t W \<noteq> None")
+  case True  
+  then obtain t v where 
+    **: "tCls t = cl_committed" "tSvrs t = write_lock" "tFk t W = Some v"
+    by auto
+  moreover have "t = the_wr_t tSvrs" using assms **
+    by (auto intro: theI2)
+  ultimately show ?thesis 
+    by (auto simp add: update_kv_key_writes_all_txn_def del: equalityI)
+next
+  case False
+  then show ?thesis using assms
+    apply (auto simp add: update_kv_key_writes_all_txn_def del: equalityI)
+    by (metis (mono_tags, lifting) option.distinct(1) the_equality)
+qed
+
+
+text \<open>Writers' sequence numbers\<close>
+
+lemma vl_writers_sqns_update_kv_key_reads_all_txn [simp]:
+  assumes "vl \<noteq> []"
+  shows "vl_writers_sqns (update_kv_key_reads_all_txn tCls tSvrs tFk vl) cl = vl_writers_sqns vl cl"
+  using assms
+  by (simp add: vl_writers_sqns_def)
+
+lemma vl_writers_sqns_update_kv_key_writes_all_txn [simp]:
+  assumes "\<And>t. tSvrs t = write_lock \<Longrightarrow> (\<exists>!t. tSvrs t = write_lock)"
+  shows "vl_writers_sqns (update_kv_key_writes_all_txn tCls tSvrs tFk vl) cl = 
+         (if (\<exists>t. tCls t = cl_committed \<and> tSvrs t = write_lock \<and> tFk t W \<noteq> None \<and> get_cl t = cl) 
+         then insert (get_sn (the_wr_t tSvrs)) (vl_writers_sqns vl cl) 
+         else vl_writers_sqns vl cl)"
+proof (cases "\<exists>t. tCls t = cl_committed \<and> tSvrs t = write_lock \<and> tFk t W \<noteq> None \<and> get_cl t = cl")
+  case True
+  then obtain t v where 
+    **: "tCls t = cl_committed" "tSvrs t = write_lock" "tFk t W = Some v" "get_cl t = cl" 
+    by auto
+  moreover have "t = the_wr_t tSvrs" using assms ** 
+    by (auto intro: theI2)
+  ultimately show ?thesis using assms
+    apply (auto simp add: vl_writers_sqns_def del: equalityI)
+    by (cases "the_wr_t tSvrs") (auto)
+next
+  case False 
+  then show ?thesis using assms
+    apply (auto simp add: vl_writers_sqns_def)
+    by (metis (mono_tags, lifting) option.simps(3) the_equality txid0.sel(2))
+qed
+
+lemma vl_writers_sqns_update_kv_all_txn [simp]:
+  assumes 
+    "vl \<noteq> []"
+    "\<And>t. tSvrs t = write_lock \<Longrightarrow> (\<exists>!t. tSvrs t = write_lock)"
+  shows "vl_writers_sqns (update_kv_all_txn tCls tSvrs tFk vl) cl = 
+         (if \<exists>t. tCls t = cl_committed \<and> tSvrs t = write_lock \<and> tFk t W \<noteq> None \<and> get_cl t = cl
+          then insert (get_sn (the_wr_t tSvrs)) (vl_writers_sqns vl cl) 
+          else vl_writers_sqns vl cl)"
+  using assms
+  by (auto simp add: update_kv_all_txn_def del: equalityI)
+
+
+(********************************************************************************************)
+(********************************************************************************************)
+(********************************************************************************************)
+
 
 \<comment> \<open>Lemmas for showing transaction id freshness\<close>
 
-lemma vl_writers_sqns_reads_other_cl_inv:
+
+lemma kvs_readers_sqns_other_cl_inv:
+  assumes "KVSNonEmp s"
+    and "cl_state (cls s cl) = cl_prepared"
+    and "cl_state (cls s' cl) = cl_committed"
+    and "\<And>k. is_locked (svr_state (svrs s k) (get_txn cl s))"
+    and "other_insts_unchanged cl (cls s) (cls s')"
+    and "svrs s' = svrs s"
+    and "cl' \<noteq> cl"
+  shows "kvs_readers_sqns (kvs_of_gs s') cl' = kvs_readers_sqns (kvs_of_gs s) cl'"
+  using assms
+  by (auto simp add: kvs_of_gs_def unchanged_defs eligible_reads_def 
+                del: equalityI)
+
+(*
+lemma vl_writers_sqns_other_cl_inv:
+  assumes "KVSNonEmp s"
+    and "\<And>k. WLockInv s k"
+    and "\<And>k. WLockFpInv s k"
+    and "cl' \<noteq> cl"
+  shows "vl_writers_sqns (update_kv_key (get_txn cl s) (svr_fp (svrs s k) (get_txn cl s))
+      (full_view vl) vl) cl' = vl_writers_sqns vl cl'"
+  using assms
+  by (auto simp add: update_kv_key_def vl_writers_sqns_def)
+*)
+
+lemma kvs_writers_sqns_other_cl_inv:
+  assumes "\<And>k. WLockInv s k" and "KVSNonEmp s"
+    and "cl_state (cls s cl) = cl_prepared"
+    and "cl_state (cls s' cl) = cl_committed"
+    and "\<And>k. is_locked (svr_state (svrs s k) (get_txn cl s))"
+    and "other_insts_unchanged cl (cls s) (cls s')"
+    and "svrs s' = svrs s"
+    and "cl' \<noteq> cl"
+  shows "kvs_writers_sqns (kvs_of_gs s') cl' = kvs_writers_sqns (kvs_of_gs s) cl'"
+  using assms
+  apply (auto simp add: kvs_of_gs_def unchanged_defs del: equalityI)
+  apply (subst vl_writers_sqns_update_kv_all_txn)
+  subgoal by auto
+  subgoal by auto
+  apply (subst vl_writers_sqns_update_kv_all_txn)
+  apply (auto del: equalityI)
+  done
+
+(*
+  apply (auto simp add: kvs_writers_sqns_def kvs_of_gs_def)
+  subgoal for x k using kvs_of_gs_cl_commit[of s cl k s'] apply simp apply (rule exI[where x=k])
+    by (smt (verit) other_insts_unchanged_def vl_writers_sqns_other_cl_inv)
+  subgoal for x k using kvs_of_gs_cl_commit[of s cl k s'] apply simp apply (rule exI[where x=k])
+    by (smt (verit) other_insts_unchanged_def vl_writers_sqns_other_cl_inv)
+  done
+*)
+
+(******)
+
+lemma get_sqns_other_cl_inv:    (****** used twice in SqnInv proof below ******)
+  assumes "\<And>k. WLockInv s k" and "KVSNonEmp s"
+    and "cl_state (cls s cl) = cl_prepared"
+    and "cl_state (cls s' cl) = cl_committed"
+    and "\<And>k. is_locked (svr_state (svrs s k) (get_txn cl s))"
+    and "svr_cl_cl'_unchanged cl s s'"
+    and "cl' \<noteq> cl"
+  shows "get_sqns (kvs_of_gs s') cl' = get_sqns (kvs_of_gs s) cl'"
+  using assms 
+  apply (auto simp add: get_sqns_def kvs_writers_sqns_other_cl_inv
+                        kvs_readers_sqns_other_cl_inv svr_cl_cl'_unchanged_def del: equalityI)
+  apply (subst kvs_writers_sqns_other_cl_inv, auto)    (* why not automatic? *)
+  done
+
+(**********)
+
+(*
+lemma vl_writers_sqns_reads_other_cl_inv:   (* NOTE: does not require vl \<noteq> [] *)
   "vl_writers_sqns (update_kv_key_reads_all_txn (\<lambda>t. cl_state (cls s (get_cl t))) tSkm tFk vl) = 
    vl_writers_sqns vl"
   unfolding vl_writers_sqns_def apply (rule ext)
@@ -1340,89 +1563,12 @@ lemma vl_writers_sqns_reads_other_cl_inv:
     by (metis (lifting) nth_list_update_eq nth_list_update_neq version.select_convs(2)
         version.surjective version.update_convs(3))
   done
+*)
 
-lemma vl_readers_sqns_other_cl_inv:
-  assumes "vl \<noteq> []"
-    and "\<And>k. WLockInv s k"
-    and "\<And>k. WLockFpInv s k"
-    and "cl' \<noteq> cl"
-  shows "vl_readers_sqns (update_kv_key (get_txn cl s) (svr_fp (svrs s k) (get_txn cl s))
-      (full_view vl) vl) cl' = vl_readers_sqns vl cl'"
-  using assms
-  by (auto simp add: update_kv_key_def vl_readers_sqns_def vl_readers_update_kv_key_writes
-                     vl_readers_update_kv_key_reads full_view_elemD)
 
-lemma kvs_readers_sqns_other_cl_inv:
-  assumes "TIDFutureKm s cl" and "TIDPastKm s cl"
-    and "\<And>k. WLockInv s k" and "\<And>k. WLockFpInv s k"
-    and "\<And>k. RLockInv s k" and "\<And>k. RLockFpInv s k"
-    and "\<And>k. NoLockFpInv s k" and "KVSNonEmp s"
-    and "cl_state (cls s cl) = cl_prepared"
-    and "cl_state (cls s' cl) = cl_committed"
-    and "\<And>k. is_locked (svr_state (svrs s k) (get_txn cl s))"
-    and "other_insts_unchanged cl (cls s) (cls s')"
-    and "svrs s' = svrs s"
-    and "cl' \<noteq> cl"
-  shows "kvs_readers_sqns (kvs_of_gs s') cl' = kvs_readers_sqns (kvs_of_gs s) cl'"
-  using assms
-  apply (auto simp add: kvs_readers_sqns_def kvs_of_gs_def)
-  subgoal for x k using kvs_of_gs_cl_commit[of s cl k s'] apply (simp add: KVSNonEmp_def)
-  apply (rule exI[where x=k])
-  by (smt (verit) other_insts_unchanged_def update_kv_all_txn_non_empty vl_readers_sqns_other_cl_inv)
-  subgoal for x k using kvs_of_gs_cl_commit[of s cl k s'] apply (simp add: KVSNonEmp_def)
-  apply (rule exI[where x=k])
-    by (smt (verit) assms(10, 12, 14) other_insts_unchanged_def update_kv_all_txn_non_empty
-        vl_readers_sqns_other_cl_inv)
-  done
+text \<open>Writer sequence numbers during client commit\<close>
 
-lemma vl_writers_sqns_other_cl_inv:
-  assumes "KVSNonEmp s"
-    and "\<And>k. WLockInv s k"
-    and "\<And>k. WLockFpInv s k"
-    and "cl' \<noteq> cl"
-  shows "vl_writers_sqns (update_kv_key (get_txn cl s) (svr_fp (svrs s k) (get_txn cl s))
-      (full_view vl) vl) cl' = vl_writers_sqns vl cl'"
-  using assms
-  by (auto simp add: update_kv_key_def vl_writers_sqns_def 
-                     vl_writers_update_kv_key_reads vl_writers_update_kv_key_writes)
-
-lemma kvs_writers_sqns_other_cl_inv:
-  assumes "TIDFutureKm s cl" and "TIDPastKm s cl"
-    and "\<And>k. WLockInv s k" and "\<And>k. WLockFpInv s k"
-    and "\<And>k. RLockInv s k" and "\<And>k. RLockFpInv s k"
-    and "\<And>k. NoLockFpInv s k" and "KVSNonEmp s"
-    and "cl_state (cls s cl) = cl_prepared"
-    and "cl_state (cls s' cl) = cl_committed"
-    and "\<And>k. is_locked (svr_state (svrs s k) (get_txn cl s))"
-    and "other_insts_unchanged cl (cls s) (cls s')"
-    and "svrs s' = svrs s"
-    and "cl' \<noteq> cl"
-  shows "kvs_writers_sqns (kvs_of_gs s') cl' = kvs_writers_sqns (kvs_of_gs s) cl'"
-  using assms
-  apply (auto simp add: kvs_writers_sqns_def kvs_of_gs_def)
-  subgoal for x k using kvs_of_gs_cl_commit[of s cl k s'] apply simp apply (rule exI[where x=k])
-    by (smt (verit) other_insts_unchanged_def vl_writers_sqns_other_cl_inv)
-  subgoal for x k using kvs_of_gs_cl_commit[of s cl k s'] apply simp apply (rule exI[where x=k])
-    by (smt (verit) other_insts_unchanged_def vl_writers_sqns_other_cl_inv)
-  done
-
-lemma get_sqns_other_cl_inv:
-  assumes "TIDFutureKm s cl" and "TIDPastKm s cl"
-    and "\<And>k. WLockInv s k" and "\<And>k. WLockFpInv s k"
-    and "\<And>k. RLockInv s k" and "\<And>k. RLockFpInv s k"
-    and "\<And>k. NoLockFpInv s k" and "KVSNonEmp s"
-    and "cl_state (cls s cl) = cl_prepared"
-    and "cl_state (cls s' cl) = cl_committed"
-    and "\<And>k. svr_state (svrs s k) (get_txn cl s) = read_lock \<or>
-             svr_state (svrs s k) (get_txn cl s) = write_lock \<or> 
-             svr_state (svrs s k) (get_txn cl s) = no_lock"
-    and "svr_cl_cl'_unchanged cl s s'"
-    and "cl' \<noteq> cl"
-  shows "get_sqns (kvs_of_gs s') cl' = get_sqns (kvs_of_gs s) cl'"
-  using assms by (auto simp add: get_sqns_def kvs_writers_sqns_other_cl_inv
-      kvs_readers_sqns_other_cl_inv cl_unchanged_defs)
-
-lemma new_t_is_in_writers:
+lemma new_t_is_in_writers_write_lock:
   assumes "TIDFutureKm s cl" and "TIDPastKm s cl"
     and "\<And>k. WLockInv s k" and "\<And>k. WLockFpInv s k"
     and "\<And>k. RLockInv s k" and "\<And>k. RLockFpInv s k"
@@ -1432,14 +1578,12 @@ lemma new_t_is_in_writers:
     and "svr_state (svrs s k) (get_txn cl s) = write_lock"
     and "other_insts_unchanged cl (cls s) (cls s')"
     and "svrs s' = svrs s"
-  shows "vl_writers_sqns (kvs_of_gs s' k) cl = vl_writers_sqns (kvs_of_gs s k) cl \<union> {cl_sn (cls s cl)}"
-  using assms kvs_of_gs_cl_commit[of s cl k s']
-  apply (auto simp add: vl_writers_sqns_def kvs_of_gs_def update_kv_key_def 
-                        vl_writers_update_kv_key_writes vl_writers_update_kv_key_reads del: equalityI)
-  apply blast   (* CHSP: what's used here? *)
-  done
+  shows "vl_writers_sqns (kvs_of_gs s' k) cl = 
+         insert (cl_sn (cls s cl)) (vl_writers_sqns (kvs_of_gs s k) cl)"
+  using assms 
+  by (auto simp add: vl_writers_sqns_def kvs_of_gs_def update_kv_key_def kvs_of_gs_cl_commit)
 
-lemma new_t_is_in_writers2:
+lemma new_t_is_in_writers_read_lock:
   assumes "TIDFutureKm s cl" and "TIDPastKm s cl"
     and "\<And>k. WLockInv s k" and "\<And>k. WLockFpInv s k"
     and "\<And>k. RLockInv s k" and "\<And>k. RLockFpInv s k"
@@ -1450,11 +1594,31 @@ lemma new_t_is_in_writers2:
     and "other_insts_unchanged cl (cls s) (cls s')"
     and "svrs s' = svrs s"
   shows "vl_writers_sqns (kvs_of_gs s' k) cl = vl_writers_sqns (kvs_of_gs s k) cl"
-  using assms kvs_of_gs_cl_commit[of s cl k s']
-  by (auto simp add: kvs_of_gs_def vl_writers_sqns_def update_kv_key_def 
-                     vl_writers_update_kv_key_reads RLockFpInv_def)
+  using assms 
+  by (auto simp add: kvs_of_gs_def vl_writers_sqns_def update_kv_key_def kvs_of_gs_cl_commit
+                     RLockFpInv_def)
 
-lemma new_t_is_in_readers:
+lemma new_t_is_in_writers_no_lock:  (* chsp added *)  (* USING update_kv_all_cl_commit_no_lock_inv *)
+  assumes "TIDFutureKm s cl" and "TIDPastKm s cl"
+    and "\<And>k. WLockInv s k" and "\<And>k. WLockFpInv s k"
+    and "\<And>k. RLockInv s k" and "\<And>k. RLockFpInv s k"
+    and "\<And>k. NoLockFpInv s k" and "KVSNonEmp s"
+    and "cl_state (cls s cl) = cl_prepared"
+    and "cl_state (cls s' cl) = cl_committed"
+    and "svr_state (svrs s k) (get_txn cl s) = no_lock"
+    and "other_insts_unchanged cl (cls s) (cls s')"
+    and "svrs s' = svrs s"
+  shows "vl_writers_sqns (kvs_of_gs s' k) cl = vl_writers_sqns (kvs_of_gs s k) cl"
+  using assms 
+  by (simp add: kvs_of_gs_def update_kv_all_cl_commit_no_lock_inv)
+
+lemmas new_t_is_in_writers_lemmas = 
+   new_t_is_in_writers_write_lock new_t_is_in_writers_read_lock new_t_is_in_writers_no_lock
+
+
+text \<open>Readers sequence numbers during client commit\<close>
+
+lemma new_t_is_in_readers_read_lock:
   assumes "TIDFutureKm s cl" and "TIDPastKm s cl"
     and "\<And>k. WLockInv s k" and "\<And>k. WLockFpInv s k"
     and "\<And>k. RLockInv s k" and "\<And>k. RLockFpInv s k"
@@ -1464,50 +1628,86 @@ lemma new_t_is_in_readers:
     and "svr_state (svrs s k) (get_txn cl s) = read_lock"
     and "other_insts_unchanged cl (cls s) (cls s')"
     and "svrs s' = svrs s"
-  shows "vl_readers_sqns (kvs_of_gs s' k) cl = vl_readers_sqns (kvs_of_gs s k) cl \<union> {cl_sn (cls s cl)}"
-  using assms kvs_of_gs_cl_commit[of s cl k s']
-  apply (auto simp add: kvs_of_gs_def update_kv_key_def vl_readers_sqns_def
-                        RLockFpInv_def KVSNonEmp_def del: equalityI)
-  (* SH does not work *)
-  sorry
+  shows "vl_readers_sqns (kvs_of_gs s' k) cl = 
+         insert (cl_sn (cls s cl)) (vl_readers_sqns (kvs_of_gs s k) cl)"
+  using assms 
 (*
-  by (meson RLockFpInv_def assms(6))
+  apply (auto simp add: kvs_of_gs_def update_kv_key_def RLockFpInv_def KVSNonEmp_def del: equalityI)
 *)
+  apply (auto simp add: kvs_of_gs_def update_kv_key_def vl_readers_sqns_def kvs_of_gs_cl_commit
+                        RLockFpInv_def KVSNonEmp_def)
+  (*
+    same problem as above: RLockFpInv is not applied (two quantifiers to instantiate)
+    NOTE: using fastforce instead of auto above works here, but should possibly improve the way 
+    in which invariants are applied.
+  *)
+  apply fastforce
+  done
 
-lemma new_t_is_in_readers2:
-  assumes "TIDFutureKm s cl" and "TIDPastKm s cl"
-    and "\<And>k. WLockInv s k" and "\<And>k. WLockFpInv s k"
-    and "\<And>k. RLockInv s k" and "\<And>k. RLockFpInv s k"
-    and "\<And>k. NoLockFpInv s k" and "KVSNonEmp s"
+
+(********)
+
+lemma eligible_reads_write_lock_no_read:
+  assumes "\<And>k. WLockInv s k" and "\<And>k. RLockInv s k" 
     and "cl_state (cls s cl) = cl_prepared"
     and "cl_state (cls s' cl) = cl_committed"
     and "svr_state (svrs s k) (get_txn cl s) = write_lock"
     and "svr_fp (svrs s k) (get_txn cl s) R \<noteq> None"
     and "other_insts_unchanged cl (cls s) (cls s')"
+  shows "eligible_reads (\<lambda>t. cl_state (cls s' (get_cl t))) (svr_state (svrs s k)) (svr_fp (svrs s k))
+       = insert (get_txn cl s) 
+           (eligible_reads (\<lambda>t. cl_state (cls s (get_cl t))) (svr_state (svrs s k)) (svr_fp (svrs s k)))"
+  using assms
+  by (auto simp add: eligible_reads_def other_insts_unchanged_def) (blast, blast, metis)
+
+
+(*******)
+
+lemma new_t_is_in_readers_write_lock:      (* chsp: using kvs_of_gs_cl_commit *)
+  assumes "TIDFutureKm s cl" and "TIDPastKm s cl"
+    and "\<And>k. WLockInv s k" and "\<And>k. WLockFpInv s k"
+    and "\<And>k. RLockInv s k" and "\<And>k. RLockFpInv s k"
+    and "\<And>k. NoLockFpInv s k" and "KVSNonEmp s"  
+    and "cl_state (cls s cl) = cl_prepared"
+    and "cl_state (cls s' cl) = cl_committed"
+    and "svr_state (svrs s k) (get_txn cl s) = write_lock"
+    and "other_insts_unchanged cl (cls s) (cls s')"
     and "svrs s' = svrs s"
-  shows "vl_readers_sqns (kvs_of_gs s' k) cl = vl_readers_sqns (kvs_of_gs s k) cl \<union> {cl_sn (cls s cl)}"
-  using assms kvs_of_gs_cl_commit[of s cl k s']
-  apply (auto simp add: kvs_of_gs_def update_kv_key_def vl_readers_sqns_def
-                        vl_readers_update_kv_key_writes split: if_split del: equalityI)
+  shows "vl_readers_sqns (kvs_of_gs s' k) cl =
+         (if svr_fp (svrs s k) (get_txn cl s) R = None
+          then vl_readers_sqns (kvs_of_gs s k) cl
+          else insert (cl_sn (cls s cl)) (vl_readers_sqns (kvs_of_gs s k) cl))"
+proof (cases "svr_fp (svrs s k) (get_txn cl s) R = None")
+  case True
+  then show ?thesis using assms 
+    by (auto simp add: kvs_of_gs_def update_kv_key_def vl_readers_sqns_def kvs_of_gs_cl_commit)
+next
+  case False
+  then show ?thesis using assms 
+    by (auto simp add: kvs_of_gs_def KVSNonEmp_def eligible_reads_write_lock_no_read
+             del: equalityI)
+       (blast)
+qed
 
-  (* SH does not work *)
-  sorry
-
-lemma new_t_is_in_readers3:
+lemma new_t_is_in_readers_no_lock:   (* chsp added *)  (* USING update_kv_all_cl_commit_no_lock_inv*)
   assumes "TIDFutureKm s cl" and "TIDPastKm s cl"
     and "\<And>k. WLockInv s k" and "\<And>k. WLockFpInv s k"
     and "\<And>k. RLockInv s k" and "\<And>k. RLockFpInv s k"
     and "\<And>k. NoLockFpInv s k" and "KVSNonEmp s"
     and "cl_state (cls s cl) = cl_prepared"
     and "cl_state (cls s' cl) = cl_committed"
-    and "svr_state (svrs s k) (get_txn cl s) = write_lock"
-    and "svr_fp (svrs s k) (get_txn cl s) R = None"
+    and "svr_state (svrs s k) (get_txn cl s) = no_lock"
     and "other_insts_unchanged cl (cls s) (cls s')"
     and "svrs s' = svrs s"
   shows "vl_readers_sqns (kvs_of_gs s' k) cl = vl_readers_sqns (kvs_of_gs s k) cl"
-  using assms kvs_of_gs_cl_commit[of s cl k s']
-  by (auto simp add: kvs_of_gs_def update_kv_key_def vl_readers_sqns_def
-                     vl_readers_update_kv_key_writes split: if_split)
+  using assms 
+  by (auto simp add: kvs_of_gs_def update_kv_all_cl_commit_no_lock_inv)
+
+lemmas new_t_is_in_readers_lemmas = 
+  new_t_is_in_readers_read_lock new_t_is_in_readers_write_lock new_t_is_in_readers_no_lock
+
+
+(***********)
 
 lemma kvs_writers_cl_commit_grows:
   assumes "TIDFutureKm s cl" and "TIDPastKm s cl"
@@ -1520,19 +1720,25 @@ lemma kvs_writers_cl_commit_grows:
     and "svr_state (svrs s k) (get_txn cl s) = write_lock"
     and "other_insts_unchanged cl (cls s) (cls s')"
     and "svrs s' = svrs s"
-  shows "kvs_writers_sqns (kvs_of_gs s') cl = kvs_writers_sqns (kvs_of_gs s) cl \<union> {cl_sn (cls s cl)}"
-  using assms new_t_is_in_writers[of s cl s' k]
-  apply (auto simp add: kvs_writers_sqns_def)
-  subgoal for x k' apply (auto elim!: allE[where x=k']; cases "k' = k", simp_all)
-    apply (metis kvs_of_gs_def read_only_update' vl_writers_sqns_reads_other_cl_inv)
-    apply (metis Un_empty_right Un_insert_right assms(3-7) insert_iff new_t_is_in_writers)
-    by (metis kvs_of_gs_def update_kv_all_cl_commit_no_lock_inv)
-  subgoal for x k' apply (rule exI[where x=k'])
-    by (smt (verit, ccfv_SIG) UnCI assms(13) kvs_of_gs_def new_t_is_in_writers new_t_is_in_writers2
-        update_kv_all_cl_commit_no_lock_inv)
-  done
+  shows "kvs_writers_sqns (kvs_of_gs s') cl = 
+         insert (cl_sn (cls s cl)) (kvs_writers_sqns (kvs_of_gs s) cl)"
+proof (intro kvs_writers_sqns_eq_insert[where k = k])
+  show "vl_writers_sqns (kvs_of_gs s' k) cl = insert (cl_sn (cls s cl)) (vl_writers_sqns (kvs_of_gs s k) cl)"
+    using assms
+    by (simp add: new_t_is_in_writers_write_lock)
+next
+  fix k'
+  have "svr_state (svrs s k') (get_txn cl s) = read_lock \<or>
+        svr_state (svrs s k') (get_txn cl s) = write_lock \<or>
+        svr_state (svrs s k') (get_txn cl s) = no_lock " using assms by simp
+  then show 
+    "vl_writers_sqns (kvs_of_gs s' k') cl = insert (cl_sn (cls s cl)) (vl_writers_sqns (kvs_of_gs s k') cl) \<or> 
+     vl_writers_sqns (kvs_of_gs s' k') cl = vl_writers_sqns (kvs_of_gs s k') cl" 
+    using assms
+    by (elim disjE) (simp_all add: new_t_is_in_writers_lemmas)
+qed
 
-lemma kvs_writers_cl_commit_doesnt_grow:
+lemma kvs_writers_cl_commit_doesnt_grow:   (* TODO: REVIEW PROOF *)
   assumes "TIDFutureKm s cl" and "TIDPastKm s cl"
     and "\<And>k. WLockInv s k" and "\<And>k. WLockFpInv s k"
     and "\<And>k. RLockInv s k" and "\<And>k. RLockFpInv s k"
@@ -1543,14 +1749,17 @@ lemma kvs_writers_cl_commit_doesnt_grow:
     and "other_insts_unchanged cl (cls s) (cls s')"
     and "svrs s' = svrs s"
   shows "kvs_writers_sqns (kvs_of_gs s') cl = kvs_writers_sqns (kvs_of_gs s) cl"
-  using assms apply (auto simp add: kvs_writers_sqns_def)
-  subgoal for x k apply (auto elim!: allE[where x=k])
-    apply (metis assms(3-7) new_t_is_in_writers2)
-    by (metis kvs_of_gs_def update_kv_all_cl_commit_no_lock_inv)
-  subgoal for x k  apply (auto elim!: allE[where x=k])
-    apply (metis assms(3-7) new_t_is_in_writers2)
-    by (metis kvs_of_gs_def update_kv_all_cl_commit_no_lock_inv)
-  done
+  using assms 
+  apply (auto simp add: kvs_of_gs_def cl_unchanged_defs del: equalityI) 
+  apply (subst vl_writers_sqns_update_kv_all_txn)
+  subgoal by auto
+  subgoal by auto
+  apply (subst vl_writers_sqns_update_kv_all_txn)
+  subgoal by auto
+  subgoal by auto
+  apply (auto del: equalityI)
+  by (metis RLockInv_def insertE other_sn_idle singletonD state_svr.distinct(5) 
+            state_svr.simps(38) state_svr.simps(42) state_svr.simps(44) txid0.collapse)
 
 lemma kvs_readers_sqns_cl_commit_grows:
   assumes "TIDFutureKm s cl" and "TIDPastKm s cl"
@@ -1565,30 +1774,23 @@ lemma kvs_readers_sqns_cl_commit_grows:
           svr_fp (svrs s k) (get_txn cl s) R \<noteq> None)"
     and "other_insts_unchanged cl (cls s) (cls s')"
     and "svrs s' = svrs s"
-  shows "kvs_readers_sqns (kvs_of_gs s') cl = kvs_readers_sqns (kvs_of_gs s) cl \<union> {cl_sn (cls s cl)}"
-  using assms
-  apply (auto simp add: kvs_readers_sqns_def del: disjE)
-  subgoal for x k' apply (auto elim!: allE[where x=k'])
-    apply (metis (no_types) Un_insert_right assms(3-7) insert_iff new_t_is_in_readers sup_bot_right)
-    apply (metis (no_types) Un_insert_right assms(3-7) insert_iff new_t_is_in_readers2
-      new_t_is_in_readers3 sup_bot_right)
-    apply (metis kvs_of_gs_def update_kv_all_cl_commit_no_lock_inv)
-    apply (metis (no_types) Un_insert_right assms(3-7) insert_iff new_t_is_in_readers sup_bot_right)
-    apply (metis (no_types) Un_insert_right assms(3-7) insert_iff new_t_is_in_readers2
-      new_t_is_in_readers3 sup_bot_right)
-    by (metis kvs_of_gs_def update_kv_all_cl_commit_no_lock_inv)
-   subgoal apply (rule exI[where x=k])
-     by (metis UnI2 assms(12,13) new_t_is_in_readers new_t_is_in_readers2 singletonI)
-   subgoal for x k' apply (auto elim!: allE[where x=k'])
-     apply (metis Un_iff assms(3-7) new_t_is_in_readers)
-     apply (smt (verit) Un_insert_left assms(3-7) insert_iff mk_disjoint_insert
-       new_t_is_in_readers2 new_t_is_in_readers3)
-     apply (metis kvs_of_gs_def update_kv_all_cl_commit_no_lock_inv)
-     apply (metis Un_iff assms(3-7) new_t_is_in_readers)
-     apply (smt (verit) Un_insert_left assms(3-7) insert_iff mk_disjoint_insert
-       new_t_is_in_readers2 new_t_is_in_readers3)
-     by (metis kvs_of_gs_def update_kv_all_cl_commit_no_lock_inv)
-   done
+  shows "kvs_readers_sqns (kvs_of_gs s') cl = 
+         insert (cl_sn (cls s cl)) (kvs_readers_sqns (kvs_of_gs s) cl)"
+proof (intro kvs_readers_sqns_eq_insert[where k=k])
+  show "vl_readers_sqns (kvs_of_gs s' k) cl = insert (cl_sn (cls s cl)) (vl_readers_sqns (kvs_of_gs s k) cl)" 
+    using assms
+    by (auto simp add: new_t_is_in_readers_lemmas del: equalityI)
+next 
+  fix k'
+  have "svr_state (svrs s k') (get_txn cl s) = read_lock \<or>
+        svr_state (svrs s k') (get_txn cl s) = write_lock \<or>
+        svr_state (svrs s k') (get_txn cl s) = no_lock " using assms by simp
+  then show 
+    "vl_readers_sqns (kvs_of_gs s' k') cl = insert (cl_sn (cls s cl)) (vl_readers_sqns (kvs_of_gs s k') cl) \<or> 
+     vl_readers_sqns (kvs_of_gs s' k') cl = vl_readers_sqns (kvs_of_gs s k') cl "
+    using assms(1-11,13,14)
+    by (elim disjE) (simp_all add: new_t_is_in_readers_lemmas)
+qed
 
 lemma kvs_readers_sqns_cl_commit_doesnt_grow:
   assumes "TIDFutureKm s cl" and "TIDPastKm s cl"
@@ -1597,22 +1799,27 @@ lemma kvs_readers_sqns_cl_commit_doesnt_grow:
     and "\<And>k. NoLockFpInv s k" and "KVSNonEmp s"
     and "cl_state (cls s cl) = cl_prepared"
     and "cl_state (cls s' cl) = cl_committed"
-    and "\<forall>k. svr_state (svrs s k) (get_txn cl s) \<in> {write_lock, no_lock}"
-    and "\<forall>k. svr_state (svrs s k) (get_txn cl s) \<noteq> write_lock \<or>
-             svr_fp (svrs s k) (get_txn cl s) R = None"
+    and "\<And>k. svr_state (svrs s k) (get_txn cl s) = no_lock \<or>
+             (svr_state (svrs s k) (get_txn cl s) = write_lock \<and>
+              svr_fp (svrs s k) (get_txn cl s) R = None)"
     and "other_insts_unchanged cl (cls s) (cls s')"
     and "svrs s' = svrs s"
   shows "kvs_readers_sqns (kvs_of_gs s') cl = kvs_readers_sqns (kvs_of_gs s) cl"
-  using assms apply (auto simp add: kvs_readers_sqns_def)
-  subgoal for x k apply (auto elim!: allE[where x=k])
-    apply (metis assms(1, 3-7) new_t_is_in_readers3)
-    by (metis kvs_of_gs_def update_kv_all_cl_commit_no_lock_inv)+
-  subgoal for x k  apply (auto elim!: allE[where x=k])
-    apply (metis assms(1, 3-7) new_t_is_in_readers3)
-    by (metis kvs_of_gs_def update_kv_all_cl_commit_no_lock_inv)+
-  done
+  using assms
+proof (intro kvs_readers_sqns_eq)
+  fix k
+  have "svr_state (svrs s k) (get_txn cl s) = no_lock \<or>
+             (svr_state (svrs s k) (get_txn cl s) = write_lock \<and>
+              svr_fp (svrs s k) (get_txn cl s) R = None)" using assms by simp
+  then show "vl_readers_sqns (kvs_of_gs s' k) cl = vl_readers_sqns (kvs_of_gs s k) cl"
+    using assms
+    by (elim disjE) (auto simp add: new_t_is_in_readers_lemmas del: equalityI)
+qed
 
-lemma get_sqns_cl_commit_grows:
+
+(********************************************************************************************)
+
+lemma get_sqns_cl_commit_grows:   (* used in SqnInv proof below *)
   assumes "TIDFutureKm s cl" and "TIDPastKm s cl"
     and "\<And>k. WLockInv s k" and "\<And>k. WLockFpInv s k"
     and "\<And>k. RLockInv s k" and "\<And>k. RLockFpInv s k"
@@ -1625,17 +1832,30 @@ lemma get_sqns_cl_commit_grows:
   shows "get_sqns (kvs_of_gs s') cl =
          (if \<forall>k. svr_state (svrs s k) (get_txn cl s) = no_lock then
           get_sqns (kvs_of_gs s) cl else
-          get_sqns (kvs_of_gs s) cl \<union> {cl_sn (cls s cl)})"
-  using assms
-  apply (cases "\<forall>k. svr_state (svrs s k) (get_txn cl s) = no_lock")
-   apply (simp add: kvs_of_gs_def update_kv_all_cl_commit_no_lock_inv)
+          insert (cl_sn (cls s cl)) (get_sqns (kvs_of_gs s) cl))" 
+proof (cases "\<forall>k. svr_state (svrs s k) (get_txn cl s) = no_lock")
+  case True
+  then show ?thesis using assms
+    apply (simp add: get_sqns_def)
+    apply (simp add:  kvs_of_gs_def)
+    by (simp add: kvs_of_gs_def update_kv_all_cl_commit_no_lock_inv)
+next
+  case False
+  then show ?thesis using assms 
   apply simp apply (rule conjI) apply blast
-  apply (simp add: get_sqns_def)
+  apply (clarsimp simp add: get_sqns_def)
   using kvs_readers_sqns_cl_commit_doesnt_grow[of s cl s']
         kvs_readers_sqns_cl_commit_grows[of s cl s']
         kvs_writers_cl_commit_doesnt_grow[of s cl s']
         kvs_writers_cl_commit_grows[of s cl s']
-  by (smt (z3) Un_insert_right insertCI sup.right_idem sup_bot_right sup_commute)
+  by (smt (verit) Un_insert_left Un_insert_right insert_absorb2 insert_iff)
+qed
+
+(********************************************************************************************)
+(********************************************************************************************)
+(********************************************************************************************)
+
+
 
 definition SqnInv where
   "SqnInv s cl \<longleftrightarrow>
@@ -1655,7 +1875,7 @@ proof(induction s arbitrary: cl rule: reach.induct)
     apply (auto simp add: SqnInv_def tps_defs kvs_of_gs_def get_sqns_old_def kvs_txids_def
         update_kv_all_defs full_view_def version_init_def)
     apply (auto simp add: kvs_writers_def vl_writers_def)
-    by (auto simp add: kvs_readers_def vl_readers_def)
+    by (auto simp add: kvs_readers_def vl_readers_def eligible_reads_def)
 next
   case (reach_trans s e s')
   then show ?case using kvs_of_gs_inv[of s e s']
@@ -1676,17 +1896,21 @@ next
   next
     case (Cl_Commit x1 x2 x3 x4)
     then show ?case
-      apply (auto simp add: SqnInv_def tps_trans_defs) using get_sqns_other_cl_inv
-      apply (smt (verit) cl_unchanged_defs reach_kvs_non_emp reach_nolockfp reach_rlock
-          reach_rlockfp reach_tidfuturekm reach_tidpastkm reach_wlock reach_wlockfp)
-      apply (cases "cl = x1")
-      using get_sqns_cl_commit_grows[of s cl s']
-      apply (smt (z3) cl_unchanged_defs UnE insert_absorb insert_iff insert_not_empty order.strict_implies_order
-        order_class.order_eq_iff other_insts_unchanged_def reach_kvs_non_emp reach_nolockfp
-        reach_rlock reach_rlockfp reach_tidfuturekm reach_tidpastkm reach_wlock reach_wlockfp)
-      using get_sqns_other_cl_inv
-      by (smt (verit) cl_unchanged_defs reach_kvs_non_emp reach_nolockfp reach_rlock
-          reach_rlockfp reach_tidfuturekm reach_tidpastkm reach_wlock reach_wlockfp)
+      apply (auto simp add: SqnInv_def tps_trans_defs) 
+      subgoal using get_sqns_other_cl_inv
+        by (smt (verit) insertCI other_insts_unchanged_def reach_kvs_non_emp reach_wlock 
+                 svr_cl_cl'_unchanged_def)
+      subgoal 
+        apply (cases "cl = x1")
+        subgoal using get_sqns_cl_commit_grows[of s cl s']
+          by (metis dual_order.eq_iff insert_iff nless_le reach_kvs_non_emp reach_nolockfp 
+                    reach_rlock reach_rlockfp reach_tidfuturekm reach_tidpastkm reach_wlock 
+                    reach_wlockfp svr_cl_cl'_unchanged_def)
+        subgoal using get_sqns_other_cl_inv
+          by (smt (verit, ccfv_SIG) insertCI other_insts_unchanged_def reach_kvs_non_emp 
+                  reach_wlock svr_cl_cl'_unchanged_def)
+        done
+      done
   next
     case (Cl_Abort x)
     then show ?case apply (auto simp add: SqnInv_def tps_trans_defs cl_unchanged_defs)
@@ -1732,7 +1956,7 @@ lemma kvs_of_gs_version_order:
    using cl_commit_updates_kv_reads[of s s' cl k] 
      expanding_feature3'[where vl="update_kv_key_reads_all_txn (\<lambda>t. cl_state (cls s (get_cl t)))
       (svr_state (svrs s k)) (svr_fp (svrs s k)) (svr_vl (svrs s k))"]
-   by (auto simp add: update_kv_key_reads_all_defs)
+   by (auto simp add: update_kv_key_reads_all_defs)    (* very slow: ~30s *)
 
 lemma new_writer:
   assumes "WLockInv s k" and "WLockFpInv s k"
@@ -1798,7 +2022,7 @@ lemma kvs_of_gs_view_atomic:
     using update_kv_all_txn_v_writer_inv[of i
         "update_kv_all_txn (\<lambda>t. cl_state (cls s (get_cl t))) (svr_state (svrs s k))
           (svr_fp (svrs s k)) (svr_vl (svrs s k))"] assms(3, 5, 6, 11)
-    apply (auto elim!: allE[where x=k])
+    apply (auto elim!: allE[where x=k])     (* very slow: ~ 25s *)
     apply (simp_all add: update_kv_all_cl_commit_no_lock_inv)
     by (metis t_is_fresh fresh_txid_v_writer kvs_of_gs_def)+
   done
@@ -1898,18 +2122,18 @@ lemma view_in_range_full_view [simp, intro]:
 lemmas view_in_range_full_view' [simp, intro] = view_in_range_full_view [unfolded o_def]
 *)
 
-lemma in_full_view_writers [simp, intro]:
+lemma in_full_view_writers:    (* To: Key_Value_Stores *)
   "\<lbrakk> i \<in> full_view (K k) \<rbrakk> \<Longrightarrow> v_writer (K k ! i) \<in> kvs_writers K"
   by (auto simp add: kvs_writers_def vl_writers_def intro: exI[where x=k])  (* uses list_nth_in_set *)
 
 
-lemma WW_relates_writers:
+lemma WW_relates_writers:      (* To: Execution_Tests *)
   "\<lbrakk> (t1, t2) \<in> WW K k \<rbrakk> \<Longrightarrow> t1 \<in> kvs_writers K \<and> t2 \<in> kvs_writers K"
-  by (auto simp add: WW_def)
+  by (auto simp add: WW_def in_full_view_writers)
 
 (*************)
 
-
+(* To: Execution_Tests? *)
 lemma R_SER_closed_simplified: "((R_SER K)\<inverse>)\<^sup>+ `` kvs_writers K \<subseteq> kvs_txids K"
 proof -
   {
@@ -1926,15 +2150,15 @@ lemma full_view_satisfies_ET_SER_canCommit: "ET_SER.canCommit K (full_view o K) 
                 all_writers_visible R_SER_closed_simplified)
 
 
-definition invariant_list where
+definition invariant_list where   (* chsp removed: KVSGSNonEmp s (derivable) *)
   "invariant_list s \<equiv> (\<forall>cl k. TIDFutureKm s cl \<and> TIDPastKm s cl \<and> RLockInv s k \<and> WLockInv s k \<and>
-    RLockFpInv s k \<and> WLockFpInv s k \<and> NoLockFpInv s k \<and> KVSNonEmp s \<and> KVSGSNonEmp s \<and>
+    RLockFpInv s k \<and> WLockFpInv s k \<and> NoLockFpInv s k \<and> KVSNonEmp s \<and> 
     RLockFpContentInv s k \<and> WLockFpContentInv s k \<and> TMFullView s cl \<and> KVSView s cl \<and> SqnInv s cl)"
 
-lemma invariant_listE [elim]:
+lemma invariant_listE [elim]:   (* chsp removed: KVSGSNonEmp s *)
  "\<lbrakk> invariant_list s; 
     \<lbrakk> \<And>cl. TIDFutureKm s cl; \<And>cl. TIDPastKm s cl; \<And>k. RLockInv s k; \<And>k. WLockInv s k;
-      \<And>k. RLockFpInv s k; \<And>k. WLockFpInv s k; \<And>k. NoLockFpInv s k; KVSNonEmp s; KVSGSNonEmp s;
+      \<And>k. RLockFpInv s k; \<And>k. WLockFpInv s k; \<And>k. NoLockFpInv s k; KVSNonEmp s; 
       \<And>k. RLockFpContentInv s k; \<And>k. WLockFpContentInv s k; 
       \<And>cl. TMFullView s cl; \<And>cl. KVSView s cl; \<And>cl. SqnInv s cl \<rbrakk> \<Longrightarrow> P \<rbrakk> 
   \<Longrightarrow> P"
@@ -1947,8 +2171,8 @@ proof (intro simulate_ES_fun_with_invariant[where I="invariant_list"])
   fix gs0 :: "'v global_conf"
   assume p: "init tps gs0"
   then show "init ET_SER.ET_ES (sim gs0)"
-    by (auto simp add: ET_SER.ET_ES_defs tps_defs sim_defs update_kv_all_defs
-        full_view_def kvs_init_def v_list_init_def lessThan_Suc)
+    by (auto simp add: ET_SER.ET_ES_defs tps_defs sim_defs update_kv_all_defs full_view_def 
+                       kvs_init_def v_list_init_def eligible_reads_def lessThan_Suc)
 next
   fix gs a and gs' :: "'v global_conf"
   assume p: "tps: gs\<midarrow>a\<rightarrow> gs'" and inv: "invariant_list gs"
@@ -1964,13 +2188,13 @@ next
                 (kvs_of_gs gs, views_of_gs gs) (ET cl sn u'' F) (kvs_of_gs gs', views_of_gs gs')\<close>
         proof (rule ET_SER.ET_trans_rule [where u'="full_view o (kvs_of_gs gs')"])
           show \<open>views_of_gs gs cl \<sqsubseteq> u''\<close> using cmt I
-            by (auto simp add: cl_commit_def views_of_gs_def elim!: TMFullViewE)
+            by (auto 4 3 simp add: cl_commit_def views_of_gs_def)
         next 
           show \<open>ET_SER.canCommit (kvs_of_gs gs) u'' F\<close> using cmt I 
             by (auto simp add: cl_commit_def full_view_satisfies_ET_SER_canCommit)
         next 
           show \<open>view_wellformed (kvs_of_gs gs) u''\<close> using cmt I
-            by (auto simp add: cl_commit_def full_view_wellformed elim!: KVSGSNonEmpE)
+            by (auto 4 4 simp add: cl_commit_def full_view_wellformed)
         next 
           show \<open>view_wellformed (kvs_of_gs gs') (full_view o (kvs_of_gs gs'))\<close> using cmt I
           proof - 
@@ -2000,8 +2224,8 @@ next
             done
         next 
           show \<open>kvs_of_gs gs' = update_kv (Tn_cl sn cl) F u'' (kvs_of_gs gs)\<close> using cmt I
-            by (auto simp add: cl_commit_def kvs_of_gs_def update_kv_def 
-                               kvs_of_gs_cl_commit svr_cl_cl'_unchanged_def)
+            by (auto 4 3 simp add: cl_commit_def kvs_of_gs_def update_kv_def 
+                                   kvs_of_gs_cl_commit svr_cl_cl'_unchanged_def)         
         next 
           show \<open>views_of_gs gs' = (views_of_gs gs)(cl := full_view o (kvs_of_gs gs'))\<close> using cmt I
             apply (auto simp add: cl_commit_def views_of_gs_def)
